implement TaggedComp.compile

src/TaggedComp.v
@@ -1,58 +1,220 @@
 Require Import List.
 Import ListNotations.
+Require Import StructTact.StructTactics.
+Require Import Omega.
 
-Require Untyped.
+Require Import Monads.
+Require Utopia.
+
+Require Lifted.
 Require Tagged.
 
-Module U := Untyped.
+Module L := Lifted.
 Module T := Tagged.
 
 
-Definition bind_option {A B : Type} (m : option A) (k : A -> option B) : option B :=
-    match m with
-    | Some x => k x
-    | None => None
+Section compile.
+Open Scope option_monad.
+
+Definition mk_rec_info ctor :=
+    let fix go acc n :=
+        match n with
+        | 0 => acc
+        | S n => go (Utopia.ctor_arg_is_recursive ctor n :: acc) n
+        end in
+    go [] (Utopia.constructor_arg_n ctor).
+
+Fixpoint mk_tagged_cases' ty idx cases : option (list (T.expr * T.rec_info)) :=
+    match cases with
+    | [] => Some []
+    | case :: cases =>
+            Utopia.type_constr ty idx >>= fun ctor =>
+            mk_tagged_cases' ty (S idx) cases >>= fun cases' =>
+            Some ((case, mk_rec_info ctor) :: cases')
     end.
 
-Notation "x '>>=' f" := (bind_option x f)
-    (at level 42, left associativity).
+Definition mk_tagged_cases ty cases :=
+    mk_tagged_cases' ty 0 cases.
 
-
-Definition fmap_option {A B : Type} (f : A -> B) (x : option A) : option B :=
-    match x with
-    | Some x => Some (f x)
-    | None => None
-    end.
-
-Notation "f <$> x" := (fmap_option f x)
-    (at level 42, left associativity).
-
-Definition seq_option {A B : Type} (f : option (A -> B)) (x : option A) : option B :=
-    match f with
-    | Some f => fmap_option f x
-    | None => None
-    end.
-
-Notation "f <*> x" := (seq_option f x)
-    (at level 42, left associativity).
-
-Fixpoint map_partial {A B : Type} (f : A -> option B) (l : list A) : option (list B) :=
-  match l with
-  | [] => Some []
-  | a :: l' => match f a, map_partial f l' with
-              | Some b, Some l'' => Some (b :: l'')
-              | _, _ => None
-              end
-  end.
-
-
-Definition zip_counter {A} (xs : list A) : list (nat * A) :=
-    let fix go i xs :=
-            match xs with
-            | [] => []
-            | x :: xs => (i, x) :: go (S i) xs
+Definition compile (e : L.expr) : option T.expr :=
+    let fix go e :=
+        let fix go_list es :=
+            match es with
+            | [] => Some []
+            | e :: es => @cons T.expr <$> go e <*> go_list es
             end in
-    go 0 xs.
+        match e with
+        | L.Arg => Some (T.Arg)
+        | L.UpVar n => Some (T.UpVar n)
+        | L.Call f a => T.Call <$> go f <*> go a
+        | L.Constr c args => T.Constr (Utopia.constructor_index c) <$> go_list args
+        | L.Elim ty cases target =>
+                go_list cases >>= fun cases =>
+                T.Elim <$> mk_tagged_cases ty cases <*> go target
+        | L.Close f free => T.Close f <$> go_list free
+        end in go e.
+
+Definition compile_list :=
+    let fix go_list (es : list L.expr) : option (list T.expr) :=
+        match es with
+        | [] => Some []
+        | e :: es => @cons T.expr <$> compile e <*> go_list es
+        end in go_list.
+
+End compile.
+
+
+
+(* Test compiler *)
+
+Eval compute in compile L.add_reflect.
+
+Definition add_comp :=
+    let x := compile L.add_reflect in
+    match x as x_ return x = x_ -> _ with
+    | Some x => fun _ => x
+    | None => fun H => ltac:(discriminate)
+    end eq_refl.
+Definition add_env_comp :=
+    let x := compile_list L.add_env in
+    match x as x_ return x = x_ -> _ with
+    | Some x => fun _ => x
+    | None => fun H => ltac:(discriminate)
+    end eq_refl.
+
+Theorem add_1_2 :
+    { x | T.star add_env_comp
+        (T.Call (T.Call add_comp (T.nat_reflect 1)) (T.nat_reflect 2)) x }.
+eexists.
+
+unfold add_comp. simpl.
+eright. eapply T.CallL, T.MakeCall; try solve [repeat econstructor].
+eright. eapply T.MakeCall; try solve [repeat econstructor].
+eright. eapply T.CallL, T.Eliminate; try solve [repeat econstructor].
+eright. eapply T.CallL, T.CallL, T.MakeCall; try solve [repeat econstructor].
+eright. eapply T.CallL, T.CallR, T.Eliminate; try solve [repeat econstructor].
+eright. eapply T.CallL, T.MakeCall; try solve [repeat econstructor].
+eright. eapply T.MakeCall; try solve [repeat econstructor].
+eright. eapply T.MakeCall; try solve [repeat econstructor].
+eleft.
+Defined.
+Eval compute in proj1_sig add_1_2.
+
+(* end of test *)
+
+
+
+
+Inductive expr_ok : L.expr -> Prop :=
+| VArg : expr_ok L.Arg
+| VUpVar : forall n, expr_ok (L.UpVar n)
+| VCall : forall f a, expr_ok f -> expr_ok a -> expr_ok (L.Call f a)
+| VConstr : forall c args,
+        Utopia.constructor_arg_n c = length args ->
+        Forall expr_ok args ->
+        expr_ok (L.Constr c args)
+| VElim : forall ty cases target,
+        (forall i, i < length cases -> Utopia.type_constr ty i <> None) ->
+        Forall expr_ok cases ->
+        expr_ok target ->
+        expr_ok (L.Elim ty cases target)
+| VClose : forall f free,
+        Forall expr_ok free ->
+        expr_ok (L.Close f free)
+.
+
+Ltac generalize_all :=
+    repeat match goal with
+    | [ y : _ |- _ ] => generalize y; clear y
+    end.
+
+(* Change the current goal to an equivalent one in which argument "x" is the
+ * first one. *)
+Tactic Notation "make_first" ident(x) :=
+    try intros until x;
+    move x at top;
+    generalize_all.
+
+(* Move "x" to the front of the goal, then perform induction. *)
+Ltac first_induction x := make_first x; induction x.
+
+Tactic Notation "intros0" ne_ident_list(xs) :=
+    intros until 0; intros xs.
+
+Notation "**" := (ltac:(eassumption)) (only parsing).
+Notation "??" := (ltac:(shelve)) (only parsing).
+
+Lemma cases_len_mk_tagged_cases' : forall ty idx cases len,
+    (forall i, i < len -> Utopia.type_constr ty i <> None) ->
+    idx + length cases = len ->
+    mk_tagged_cases' ty idx cases <> None.
+first_induction cases; intros0 Hok Hlen; simpl.
+{ discriminate. }
+compute [seq fmap bind_option]. simpl in Hlen.
+assert (idx < len) by omega.
+pose proof Hok. specialize (Hok _ **). break_match; try congruence.
+specialize (IHcases _ (S idx) _ ** ltac:(omega)). break_match; congruence.
+Qed.
+
+Lemma cases_len_mk_tagged_cases : forall ty cases,
+    (forall i, i < length cases -> Utopia.type_constr ty i <> None) ->
+    mk_tagged_cases ty cases <> None.
+intros. unfold mk_tagged_cases. eapply cases_len_mk_tagged_cases'; eauto.
+Qed.
+
+Lemma compile_list_len : forall es es',
+    compile_list es = Some es' ->
+    length es = length es'.
+induction es; intros0 Hcomp; simpl in *.
+- injection Hcomp. intro HH. rewrite <- HH. reflexivity.
+- compute [seq fmap bind_option] in Hcomp.
+  break_match; try discriminate.
+  break_match; try discriminate.
+  break_match; try discriminate.
+  invc Heqo. invc Hcomp. erewrite IHes; eauto. reflexivity.
+Qed.
+
+Theorem expr_ok_compile : forall e, expr_ok e -> compile e <> None.
+induction e using L.expr_rect_mut
+    with (Pl := fun es => Forall expr_ok es -> compile_list es <> None);
+    intros0 Hok; simpl.
+
+- discriminate.
+
+- discriminate.
+
+- compute [seq fmap bind_option].
+  invc Hok. specialize (IHe1 **). specialize (IHe2 **).
+  destruct (compile e1); try congruence.
+  destruct (compile e2); try congruence.
+
+- fold compile_list. compute [seq fmap bind_option].
+  invc Hok. specialize (IHe **).
+  break_match; congruence.
+
+- fold compile_list. compute [seq fmap bind_option].
+  invc Hok. specialize (IHe **). specialize (IHe0 **).
+  break_match; try congruence.
+  break_match; cycle 1.
+    { break_match; try discriminate.
+      contradict Heqo1. eapply cases_len_mk_tagged_cases.
+      intro. erewrite <- compile_list_len; eauto. }
+  break_match; try congruence.
+
+- fold compile_list. compute [seq fmap bind_option].
+  invc Hok. specialize (IHe **).
+  break_match; congruence.
+
+- discriminate.
+
+- compute [seq fmap bind_option].
+  invc Hok. specialize (IHe **). specialize (IHe0 **).
+  destruct (compile _); try congruence.
+  destruct (compile_list _); try congruence.
+
+Qed.
+
+
 
 (*
 Definition index_to_count ty idx_e : option (nat * T.expr) :=
